Thoughts on new restrictions of the renaming lists

src/Concurrent/Examples.v
@@ -2,6 +2,131 @@ From CoreErlang.Concurrent Require Import BarbedBisim.
 
 Import ListNotations.
 
+Definition appearsEther (ι : PID) (eth : Ether) : Prop :=
+  isUsedEther ι eth \/
+  (exists (ι' : PID), eth !! (ι, ι') ≠ None) \/
+  (exists (ιs ιd : PID) (t : list Signal),
+     eth !! (ιs, ιd) = Some t /\ ι ∈ (flat_union usedPIDsSignal t)).
+
+Proposition isUsedEther_appearsEther :
+  forall ι eth, isUsedEther ι eth -> appearsEther ι eth.
+Proof.
+  intros. by left.
+Qed.
+
+Proposition appearsEther_isUsedEther :
+  forall ι eth, ¬appearsEther ι eth -> ¬isUsedEther ι eth.
+Proof.
+  intros. intro. apply H. by apply isUsedEther_appearsEther.
+Qed.
+
+Proposition not_appearsEther_alt :
+  forall ι eth, ¬appearsEther ι eth <->
+    (
+      ¬isUsedEther ι eth /\
+      (forall ι', eth !! (ι, ι') = None) /\
+      (forall ιs ιd t, eth !! (ιs, ιd) = Some t -> ι ∉ (flat_union usedPIDsSignal t))
+    ).
+Proof.
+  intros. split; intros.
+  * intuition.
+    - apply H. by left.
+    - apply eq_None_ne_Some_2. intros. intro.
+      apply H. right. left. exists ι'. by rewrite H0.
+    - apply H. right. right.
+      apply elem_of_flat_union in H1. destruct_hyps.
+      exists ιs, ιd, t. split; auto.
+      apply elem_of_flat_union. set_solver.
+  * intro. destruct_hyps. destruct H0. congruence.
+    destruct_or!.
+    - set_solver.
+    - set_solver.
+Qed.
+
+Corollary does_not_appear_renamePID_ether :
+  forall eth p p', ¬ appearsEther p eth -> ¬ appearsEther p' eth ->
+    renamePIDEther p p' eth = eth.
+Proof.
+  intros. unfold renamePIDEther.
+  apply map_eq. intros. destruct i as [ιs ιd].
+  destruct (eth !! (ιs, ιd)) eqn:P; setoid_rewrite P.
+  {
+    apply lookup_kmap_Some; auto.
+    assert (ιs ≠ p /\ ιs ≠ p' /\ ιd ≠ p /\ ιd ≠ p'). {
+      split_and!; intro; subst.
+      * apply H. right. left. exists ιd. intro. congruence.
+      * apply H0. right. left. exists ιd. intro. congruence.
+      * apply H. left. by exists ιs, l.
+      * apply H0. left. by exists ιs, l.
+    }
+    exists (ιs, ιd). destruct_hyps. simpl.
+    unfold renamePIDPID_sym; repeat case_match; eqb_to_eq; subst; try congruence.
+    split. reflexivity.
+    rewrite lookup_fmap. setoid_rewrite P. simpl.
+    f_equal.
+    rewrite <- (map_id l) at 2.
+    apply map_ext_Forall. apply Forall_forall. intros.
+    apply isNotUsed_renamePID_signal.
+    intro. apply H. right. right. do 3 eexists. split. exact P.
+    apply elem_of_flat_union. eexists. split; eassumption.
+  }
+  {
+    apply lookup_kmap_None; auto.
+    intros. destruct i. cbn in H1. setoid_rewrite lookup_fmap.
+    unfold renamePIDPID_sym in H1.
+    repeat case_match; eqb_to_eq; subst; simpl in *; inv H1.
+    9: try by setoid_rewrite P.
+    all: try by (apply not_appearsEther_alt in H; destruct_hyps;
+      rewrite H1).
+    all: try by (apply not_appearsEther_alt in H0; destruct_hyps;
+      rewrite H1).
+    * apply not_appearsEther_alt in H; destruct_hyps.
+      unfold isUsedEther in H.
+      assert (forall ι' l, eth !! (ι', p) ≠ Some l) by set_solver.
+      eapply eq_None_ne_Some_2 in H5. by setoid_rewrite H5.
+    * apply not_appearsEther_alt in H0; destruct_hyps.
+      unfold isUsedEther in H0.
+      assert (forall ι' l, eth !! (ι', p') ≠ Some l) by set_solver.
+      eapply eq_None_ne_Some_2 in H6. by setoid_rewrite H6.
+  }
+Qed.
+
+Corollary isNotUsed_renamePID_pool :
+  forall Π p p', ¬ isUsedPool p Π -> ¬ isUsedPool p' Π ->
+    renamePIDPool p p' Π = Π.
+Proof.
+  intros. unfold renamePIDPool.
+  apply map_eq. intros.
+  destruct (Π !! i) eqn:P; setoid_rewrite P.
+  {
+    apply lookup_kmap_Some; auto.
+    assert (i ≠ p /\ i ≠ p'). {
+      split_and!; intro; subst.
+      * apply H. left. intro. congruence.
+      * apply H0. left. intro. congruence.
+    }
+    exists i. destruct_hyps. simpl.
+    unfold renamePIDPID_sym; repeat case_match; eqb_to_eq; subst; try congruence.
+    split. reflexivity.
+    rewrite lookup_fmap. setoid_rewrite P. simpl.
+    f_equal.
+    apply isNotUsed_renamePID_proc.
+    intro. apply H. right. do 2 eexists. split. exact P. assumption.
+  }
+  {
+    apply lookup_kmap_None; auto.
+    intros.
+    unfold renamePIDPID_sym in H1.
+    repeat case_match; eqb_to_eq; subst; simpl in *.
+    all: setoid_rewrite lookup_fmap.
+    3: try by setoid_rewrite P.
+    * destruct (Π !! p) eqn:Q; setoid_rewrite Q; auto.
+      exfalso. apply H. left. intro. congruence.
+    * destruct (Π !! p') eqn:Q; setoid_rewrite Q; auto.
+      exfalso. apply H0. left. intro. congruence.
+  }
+Qed.
+
 (* InductiveNodeSemantics.v *)
 (* Lemma ether_is_not_affected :
   forall n n' l, n -[l]ₙ->* n' ->
@@ -240,7 +365,7 @@ Proof.
   set_solver.
 Qed.
 
-Lemma rename_preCompatible :
+(* Lemma rename_preCompatible :
   forall O eth Π p p',
   ¬isUsedPool p' Π ->
   (* p' ∉ dom Π -> *)
@@ -275,14 +400,46 @@ Proof.
       congruence.
     }
     now apply isUsedEther_rename_same_neq.
-Qed.
+Qed. *)
 
+
+Lemma rename_preCompatible:
+  forall O eth Π p p',
+  ¬isUsedPool p' Π ->
+  (* p' ∉ dom Π -> *)
+  p' ∉ O ->
+  p ∉ O ->
+  (* ¬appearsEther p' eth -> *)
+  preCompatibleNodes O (eth, Π)
+    (renamePIDEther p p' eth, renamePIDPool p p' Π).
+Proof.
+  split; simpl.
+  * apply lookup_kmap_None; auto. intros.
+    destruct H3. unfold renamePIDPID_sym in H4. repeat case_match; eqb_to_eq; subst.
+    - simpl in *. congruence.
+    - rewrite lookup_fmap.
+      assert (Π !! p' = None). {
+        apply eq_None_ne_Some_2. intros. intro. apply H. left.
+        intro. congruence.
+      }
+      now setoid_rewrite H4.
+    - rewrite lookup_fmap. simpl in *. now setoid_rewrite H3.
+  * destruct H3. simpl in *.
+    assert (ι ≠ p'). {
+      intro. subst. congruence.
+    }
+    assert (ι ≠ p). {
+      intro. subst.
+      congruence.
+    }
+    now apply isUsedEther_rename_same_neq.
+Qed.
 
 Corollary rename_preCompatible_sym :
   forall O eth Π p p',
   ¬isUsedPool p' Π ->
   (* p' ∉ dom Π -> *)
-  ¬isUsedEther p' eth ->
+  (* ¬isUsedEther p' eth -> *)
   p' ∉ O ->
   p ∉ O ->
   (* ¬isUntaken p (eth, Π) -> *)
@@ -292,16 +449,16 @@ Proof.
   intros. split.
   * apply rename_preCompatible; auto.
   * split; simpl.
-    - destruct H4. simpl in *. setoid_rewrite lookup_kmap_None in H4; auto.
-      specialize (H4 ι). unfold renamePIDPID_sym in H4.
+    - destruct H3. simpl in *. setoid_rewrite lookup_kmap_None in H3; auto.
+      specialize (H3 ι). unfold renamePIDPID_sym in H3.
       repeat break_match_hyp; eqb_to_eq; subst.
       + simpl in *. congruence.
       + congruence.
-      + rewrite lookup_fmap in H4. simpl in *.
-        specialize (H4 eq_refl).
-        destruct (Π !! ι) eqn:P; setoid_rewrite P in H4. simpl in H4. congruence.
+      + rewrite lookup_fmap in H3. simpl in *.
+        specialize (H3 eq_refl).
+        destruct (Π !! ι) eqn:P; setoid_rewrite P in H3. simpl in H3. congruence.
         reflexivity.
-    - destruct H4. simpl in *.
+    - destruct H3. simpl in *.
       assert (ι ≠ p'). {
         intro. subst. congruence.
       }
@@ -309,7 +466,7 @@ Proof.
         intro. subst.
         congruence.
       }
-      by apply isUsedEther_rename_same_neq in H5.
+      by apply isUsedEther_rename_same_neq in H4.
 Qed.
 
 (* Lemma impossible_send :
@@ -488,47 +645,6 @@ Proof.
   
 Admitted. *)
 
-Definition appearsEther (ι : PID) (eth : Ether) : Prop :=
-  isUsedEther ι eth \/
-  (exists (ι' : PID), eth !! (ι, ι') ≠ None) \/
-  (exists (ιs ιd : PID) (t : list Signal),
-     eth !! (ιs, ιd) = Some t /\ ι ∈ (flat_union usedPIDsSignal t)).
-
-Proposition isUsedEther_appearsEther :
-  forall ι eth, isUsedEther ι eth -> appearsEther ι eth.
-Proof.
-  intros. by left.
-Qed.
-
-Proposition appearsEther_isUsedEther :
-  forall ι eth, ¬appearsEther ι eth -> ¬isUsedEther ι eth.
-Proof.
-  intros. intro. apply H. by apply isUsedEther_appearsEther.
-Qed.
-
-Proposition not_appearsEther_alt :
-  forall ι eth, ¬appearsEther ι eth <->
-    (
-      ¬isUsedEther ι eth /\
-      (forall ι', eth !! (ι, ι') = None) /\
-      (forall ιs ιd t, eth !! (ιs, ιd) = Some t -> ι ∉ (flat_union usedPIDsSignal t))
-    ).
-Proof.
-  intros. split; intros.
-  * intuition.
-    - apply H. by left.
-    - apply eq_None_ne_Some_2. intros. intro.
-      apply H. right. left. exists ι'. by rewrite H0.
-    - apply H. right. right.
-      apply elem_of_flat_union in H1. destruct_hyps.
-      exists ιs, ιd, t. split; auto.
-      apply elem_of_flat_union. set_solver.
-  * intro. destruct_hyps. destruct H0. congruence.
-    destruct_or!.
-    - set_solver.
-    - set_solver.
-Qed.
-
 Lemma fresh_pid_is_not_in_step :
   forall O n n' a ι,
   n -[ a | ι ]ₙ-> n' with O ->
@@ -536,7 +652,7 @@ Lemma fresh_pid_is_not_in_step :
     ¬ isUsedPool p' n.2 ->
     ¬ appearsEther p' n.1 ->
     p' ∉ O ->
-   p' ∉ (usedPIDsAct a) \/ (exists v1 v2, a = ASpawn p' v1 v2)).
+   p' ∉ (usedPIDsAct a) \/ (exists v1 v2, a = ASpawn p' v1 v2 /\ p' ∉ usedPIDsVal v1 ∪ usedPIDsVal v2)).
 Proof.
   intros. inv H; simpl in *. 1-3: left; intro.
   * assert (p' = ι \/ (p' = ι' \/ p' ∈ usedPIDsSignal t)) by set_solver.
@@ -557,7 +673,9 @@ Proof.
     apply H0. left. assert (p' = ι) by set_solver. subst.
     by setoid_rewrite lookup_insert.
   * destruct (decide (ι' = p')).
-    - subst. right. do 2 eexists. reflexivity.
+    - subst. right. do 2 eexists. split. reflexivity.
+      intro. apply H0. right. exists ι, p. split. by setoid_rewrite lookup_insert.
+      inv H9. set_solver.
     - left. intro.
       apply H0. right. exists ι, p. split. by setoid_rewrite lookup_insert.
       inv H9; simpl in *.
@@ -618,6 +736,8 @@ Proof.
         right. right. do 3 eexists. split; eassumption.
 Qed.
 
+(* Axiom ff : False.
+
 Theorem rename_bisim :
   forall O eth Π p p',
     ether_wf eth ->
@@ -653,7 +773,26 @@ Proof.
         + eapply not_isUsedPool_step in H4; try eassumption.
     }
     { (* p' should be renamed to a fresh variable <- not guarded anymore *)
-      admit.
+      destruct_hyps. subst.
+      assert (exists new, ¬ appearsEther new eth /\ ¬isUsedPool new Π /\ new ∉ O /\
+               new ∉ usedPIDsVal x ∪ usedPIDsVal x0). {
+        exfalso. apply ff.
+      }
+      destruct H5 as [new H5]. destruct_hyps.
+      exists (renamePIDEther p p' (renamePIDEther p' new eth'), renamePIDPool p p' (renamePIDPool p' new Π')),
+             [(renamePIDAct p p' (renamePIDAct p' new  (ASpawn p' x x0)), renamePIDPID_sym p p' (renamePIDPID_sym p' new  ι))].
+      rewrite <- (does_not_appear_renamePID_ether eth p' new); auto.
+      rewrite <- (isNotUsed_renamePID_pool Π p' new); auto.
+      split.
+      eapply n_trans.
+        eapply renamePID_is_preserved_node_semantics.
+        eapply renamePID_is_preserved_node_semantics.
+        exact H4.
+        9: apply n_refl.
+        all: auto. 1-5: exfalso; apply ff.
+      eapply barbedBisim_trans. 2: apply IH. apply IH.
+      all: clear IH; try assumption.
+      all: exfalso; apply ff.
     }
   * simpl. intros.
     exists (renamePIDPID_sym p p' source), []. eexists.
@@ -682,9 +821,9 @@ Proof.
         setoid_rewrite P. simpl. trivial.
       }
     }
-  * admit.
-  * admit.
-Abort.
+  * exfalso. apply ff.
+  * exfalso. apply ff.
+Qed. *)
 
 Definition PIDRenamingList := list (PID * PID).
 Definition renamePIDs {A} (f : PID -> PID -> A -> A) (l : PIDRenamingList) (x : A) : A :=
@@ -775,48 +914,130 @@ Proof.
       rewrite n0 in H0. set_solver.
 Qed.
 
-(* Lemma isUsedPool_rename_same_new :
+Lemma isUsedPool_rename_same_new_1 :
   ∀ (p p' : PID) (Π : ProcessPool),
-    isUsedPool p Π ↔ isUsedPool p' Π .[ p ⇔ p' ]ₚₚ.
+    isUsedPool p Π -> isUsedPool p' Π .[ p ⇔ p' ]ₚₚ.
 Proof.
-  intros. split; intro.
-  {
-    destruct H.
-    * left. intro. setoid_rewrite lookup_kmap_None in H0; auto.
-      specialize (H0 p). unfold renamePIDPID_sym in H0.
-      rewrite Nat.eqb_refl in H0.
-      repeat case_match; eqb_to_eq; try congruence; subst;
-      specialize (H0 eq_refl);
-      setoid_rewrite lookup_fmap in H0.
-      - destruct (Π !! _) eqn:P; setoid_rewrite P in H0.
-        simpl in H0. congruence.
-        congruence.
-    * right.
-      destruct_hyps.
-      exists (renamePIDPID_sym p p' x), (renamePIDProc p p' x0). split.
-      - setoid_rewrite lookup_kmap; auto.
-        setoid_rewrite lookup_fmap. by setoid_rewrite H.
-      - rewrite usedPIDsProc_rename_elem_of. 2: assumption. set_solver.
-  }
-  {
-    destruct H.
-    * left. intro. apply H. apply lookup_kmap_None; auto.
-      intros. setoid_rewrite lookup_fmap.
-      unfold renamePIDPID_sym in H1. repeat case_match; eqb_to_eq; subst; try congruence.
-      by setoid_rewrite H0.
-    * right.
-      destruct_hyps.
-      setoid_rewrite lookup_kmap_Some in H; auto. destruct_hyps.
-      setoid_rewrite lookup_fmap in H1.
-      destruct (Π !! x1) eqn:P; setoid_rewrite P in H1; inv H1.
-      exists x1, p0. split.
-      - assumption.
-      - destruct (gset_elem_of_dec p (usedPIDsProc p0)). assumption.
-        WRONG
-  }
-Admitted. *)
+  intros.
+  destruct H.
+  * left. intro. setoid_rewrite lookup_kmap_None in H0; auto.
+    specialize (H0 p). unfold renamePIDPID_sym in H0.
+    rewrite Nat.eqb_refl in H0.
+    repeat case_match; eqb_to_eq; try congruence; subst;
+    specialize (H0 eq_refl);
+    setoid_rewrite lookup_fmap in H0.
+    - destruct (Π !! _) eqn:P; setoid_rewrite P in H0.
+      simpl in H0. congruence.
+      congruence.
+  * right.
+    destruct_hyps.
+    exists (renamePIDPID_sym p p' x), (renamePIDProc p p' x0). split.
+    - setoid_rewrite lookup_kmap; auto.
+      setoid_rewrite lookup_fmap. by setoid_rewrite H.
+    - rewrite usedPIDsProc_rename_elem_of. 2: assumption. set_solver.
+Qed.
+
+Lemma isUsedPool_rename_same_new_2 :
+  ∀ (p p' : PID) (Π : ProcessPool),
+    ¬isUsedPool p' Π ->
+    isUsedPool p' Π .[ p ⇔ p' ]ₚₚ -> isUsedPool p Π.
+Proof.
+  intros.
+  destruct H0.
+  * left. intro. apply H0. apply lookup_kmap_None; auto.
+    intros. setoid_rewrite lookup_fmap.
+    unfold renamePIDPID_sym in H2. repeat case_match; eqb_to_eq; subst; try congruence.
+    by setoid_rewrite H1.
+  * right.
+    destruct_hyps.
+    setoid_rewrite lookup_kmap_Some in H0; auto. destruct_hyps.
+    setoid_rewrite lookup_fmap in H2.
+    destruct (Π !! x1) eqn:P; setoid_rewrite P in H2; inv H2.
+    exists x1, p0. split.
+    - assumption.
+    - destruct (gset_elem_of_dec p (usedPIDsProc p0)). assumption.
+      assert (p' ∉ usedPIDsProc p0). {
+        intro. apply H. right. do 2 eexists. split; eassumption.
+      }
+      rewrite isNotUsed_renamePID_proc in H1; auto.
+      congruence.
+Qed.
+
+(*
+  If something is renamed, then it should not be renamed again
+  if the ith element of the list is (from, to) then from should not appear 
+
+*)
+
+Inductive well_formed (O : gset PID) : Node -> list (PID * PID) -> Prop :=
+| wf_nil Π : well_formed O Π nil
+| wf_cons eth Π l from to:
+  well_formed O (renamePIDEther from to eth, renamePIDPool from to Π) l ->
+  from ∉ O ->
+  to ∉ O ->
+  ¬isUsedPool to Π ->
+  ¬appearsEther to eth
+->
+  well_formed O (eth, Π) ((from, to) :: l).
 
 Corollary renameList_preCompatible_sym :
+  forall O l eth Π,
+  (* ¬isUsedPool p' Π ->
+  (* p' ∉ dom Π -> *)
+  ¬isUsedEther p' eth ->
+  p' ∉ O ->
+  p ∉ O -> *)
+  (* Forall (fun '(from, to) => (* ¬ appearsEther to eth /\ *) ¬isUsedPool to Π
+     /\ to ∉ O /\ from ∉ O) l ->
+  NoDup (map fst l) -> *)
+  well_formed O (eth, Π) l ->
+  (* ¬isUntaken p (eth, Π) -> *)
+  symClos (preCompatibleNodes O) (eth, Π)
+    (renamePIDs renamePIDEther l eth, renamePIDs renamePIDPool l Π).
+Proof.
+  induction l; intros.
+  cbn. split; apply preCompatibleNodes_refl.
+  inv H. simpl.
+  split.
+  {
+    eapply preCompatibleNodes_trans.
+    eapply rename_preCompatible with (p := from) (p' := to). 1-3: assumption.
+    apply IHl; try assumption.
+(*     {
+      rewrite Forall_forall in H5. apply Forall_forall. intros.
+      apply H5 in H2. destruct x; simpl in *. destruct_and!.
+      split_and!; try assumption.
+      intro. apply isUsedPool_rename_same_neq in H7. congruence.
+      intro. subst. apply isUsedPool_rename_same_old in H7. congruence.
+      intro. subst. apply isUsedPool_rename_same_new_2 in H7; try assumption.
+      congruence.
+    }
+ *)
+  }
+  {
+    (* destruct_hyps. inv H0. *)
+    eapply preCompatibleNodes_trans.
+    apply IHl; try assumption.
+(*     1: {
+      admit.
+      (* clear -H H1 H4 H7 H8.
+      induction H4; constructor; auto.
+      * destruct x.
+        clear IHForall. simpl in *.
+        destruct_and!. split_and!.
+        - intro. apply isUsedEther_rename_same_neq in H5. congruence. 2: set_solver.
+          intro. subst. apply isUsedEther_rename_same_old in H5. congruence.
+        - intro. apply isUsedPool_rename_same_neq in H5. congruence. 2: set_solver.
+          intro. subst. apply isUsedPool_rename_same_old in H5. congruence.
+        - set_solver.
+        - set_solver.
+      * apply IHForall; auto. set_solver. now inv H8. *)
+    } *)
+    eapply rename_preCompatible_sym with (p := from) (p' := to). 1-3: assumption.
+  }
+Qed.
+
+Corollary renameList_preCompatible_sym_old :
   forall O l eth Π,
   (* ¬isUsedPool p' Π ->
   (* p' ∉ dom Π -> *)
@@ -836,7 +1057,7 @@ Proof.
   {
     destruct_hyps. inv H0.
     eapply preCompatibleNodes_trans.
-    eapply rename_preCompatible with (p := p) (p' := p0). 1-4: assumption.
+    eapply rename_preCompatible with (p := p) (p' := p0). 1-3: assumption.
     apply IHl; try assumption.
     {
       clear -H H1 H4 H7 H8.
@@ -868,7 +1089,7 @@ Proof.
         - set_solver.
       * apply IHForall; auto. set_solver. now inv H8.
     }
-    eapply rename_preCompatible_sym with (p := p) (p' := p0). 1-4: assumption.
+    eapply rename_preCompatible_sym with (p := p) (p' := p0). 1-3: assumption.
   }
 Qed.
 
@@ -890,34 +1111,88 @@ Proof.
     }
 Qed.
 
-Lemma fresh_pid_list_is_not_in_step :
-  forall O n n' a ι,
+(* Lemma fresh_pid_list_is_not_in_step :
+  forall l O n n' a ι,
   n -[ a | ι ]ₙ-> n' with O ->
-  (forall l,
-    Forall (fun p' => ¬ isUsedPool p' n.2 /\
-                      ¬ appearsEther p' n.1 /\
-                      p' ∉ O) l ->
-   Forall (fun p' => p' ∉ (usedPIDsAct a)) l \/
-   (exists v1 v2 p', a = ASpawn p' v1 v2 /\ p' ∈ l)).
+  (
+    well_formed O n l ->
+   Forall (fun p' => p' ∉ (usedPIDsAct a)) (map snd l) \/
+   (exists v1 v2 p', a = ASpawn p' v1 v2 /\ p' ∈ (map snd l) /\ p' ∉ usedPIDsVal v1 ∪ usedPIDsVal v2)).
 Proof.
   induction l; intros; inv H0.
   * left. constructor.
-  * destruct_and!. eapply fresh_pid_is_not_in_step in H as P; eauto.
+  * eapply fresh_pid_is_not_in_step in H as P; eauto.
     destruct P.
-    - apply IHl in H4. destruct H4.
-      + left. by constructor.
+    - destruct n' as [eth' Π']. eapply IHl with (a := renamePIDAct from to a0) in H3.
+      2: { apply renamePID_is_preserved_node_semantics; eauto.
+           by apply appearsEther_isUsedEther.
+         }
+      destruct H3.
+      + left. simpl. constructor. by simpl.
+        {
+          apply Forall_forall. rewrite Forall_forall in H1. intros.
+          apply H1 in H2.
+        }
       + destruct_hyps. subst. simpl in *.
         right. do 3 eexists. split. reflexivity.
-        set_solver.
+        split. 1: set_solver.
+        assumption.
+      + 
     - right. destruct_hyps. do 3 eexists. split. eassumption.
-      set_solver.
-Qed.
+      split. 1: set_solver. assumption.
+Qed. *)
 
+(* TODO: generalize this *)
+Fixpoint collapse_list (l : list (PID * PID)) (a : Action) :=
+match l with
+| (from, to)::l => to ∉ usedPIDsAct a /\ collapse_list l (renamePIDAct from to a)
+| [] => True
+end.
 
 Theorem renamePIDlist_is_preserved_node_semantics :
   forall l O eth eth' Π Π' a ι,
     (eth, Π) -[a | ι]ₙ-> (eth', Π') with O ->
-      Forall (fun '(from, to) => to ∉ (usedPIDsAct a) /\
+      (* Forall (fun '(from, to) => to ∉(usedPIDsAct a)(*  /\
+                                 ¬ isUsedEther to eth *) (* /\ *)
+                                 (* ¬ isUsedPool to Π /\ *)
+                                 (* to ∉ O *)) l -> *)
+      collapse_list l a ->
+      (* NoDup (map snd l) -> *)
+      well_formed O (eth, Π) l ->
+      (renamePIDs renamePIDEther l eth, renamePIDs renamePIDPool l Π)
+    -[renamePIDs renamePIDAct l a | renamePIDs renamePIDPID_sym l ι]ₙ->
+      (renamePIDs renamePIDEther l eth', renamePIDs renamePIDPool l Π') with O.
+Proof.
+  induction l; intros. by assumption.
+  destruct a. simpl. inv H1.
+  inv H0. destruct_hyps.
+  eapply IHl; auto.
+  {
+    apply renamePID_is_preserved_node_semantics; try assumption.
+    by apply appearsEther_isUsedEther.
+  }
+  (* rewrite Forall_forall in H4. apply Forall_forall. intros.
+  destruct x. apply H4 in H0 as P. simpl in *. (*  (* clear H4. *) destruct_hyps. split_and!. *)
+  * destruct (decide (p2 = p)).
+    - subst. admit. (* P -> usedPIDsAct a0.[[p->p0]] = usedPIDsAct a0 *)
+    - admit. (* This case is doable *)
+(*   * intro. apply isUsedEther_rename_same_neq in H6. congruence.
+    - intro. subst. apply isUsedEther_rename_same_old in H6.
+      congruence.
+    - intro. subst. admit.
+  * intro. apply isUsedPool_rename_same_neq in H11. congruence.
+    - intro. subst. apply isUsedPool_rename_same_old in H11.
+      congruence.
+    - intro. subst. apply H4. apply elem_of_map_iff. exists (p1, p0). split; auto.
+  * set_solver.
+ *) *)
+Qed.
+
+(*
+Theorem renamePIDlist_is_preserved_node_semantics_weakened :
+  forall l O eth eth' Π Π' a ι,
+    (eth, Π) -[a | ι]ₙ-> (eth', Π') with O ->
+      Forall (fun '(from, to) => (to ∈ (usedPIDsAct a) -> exists new, new ≠ to /\ (to, new) ∈ l /\ new ∉ (usedPIDsAct a)) /\
                                  ¬ isUsedEther to eth /\
                                  ¬ isUsedPool to Π /\
                                  to ∉ O) l ->
@@ -929,9 +1204,18 @@ Proof.
   induction l; intros. by assumption.
   destruct a. simpl. inv H1.
   inv H0. destruct_hyps.
+  destruct (gset_elem_of_dec p0 (usedPIDsAct a0)).
+  {
+    apply H0 in e. destruct e as [new [Heq [Hin Hfst]]].
+    apply elem_of_cons in Hin as [|].
+    * inv H7. congruence.
+    * simpl in Hfst.
+      (* p0 <-> new, i.e., p <-> p0 could be replaced by p <-> new *)
+      admit.
+  }
   eapply IHl; auto.
   {
-    apply renamePID_is_preserved_node_semantics; assumption.
+    apply renamePID_is_preserved_node_semantics; try assumption.
   }
   rewrite Forall_forall in H6. apply Forall_forall. intros.
   destruct x. apply H6 in H7 as H7'. simpl in *. clear H6. destruct_hyps. split_and!.
@@ -947,10 +1231,352 @@ Proof.
       congruence.
     - intro. subst. apply H4. apply elem_of_map_iff. exists (p1, p0). split; auto.
   * set_solver.
-Admitted.
+Admitted.*)
+
+Lemma well_formed_preserved :
+  forall l O n n' a ι,
+    well_formed O n l ->
+    collapse_list l a ->
+    n -[a | ι]ₙ-> n' with O ->
+    well_formed O n' l.
+Proof.
+  induction l; intros. constructor. destruct n'.
+  inv H. inv H0. eapply IHl in H4; eauto.
+  2: { eapply renamePID_is_preserved_node_semantics. exact H1.
+       all: try assumption.
+       by apply appearsEther_isUsedEther.
+     }
+  constructor; auto.
+  * eapply not_isUsedPool_step; eauto.
+  * eapply appearsEther_step in H1; eauto.
+Qed.
+
+Lemma renamePIDPID_1 :
+  forall a b, renamePIDPID a b a = b.
+Proof.
+  unfold renamePIDPID. intros. by rewrite Nat.eqb_refl.
+Qed.
+
+Lemma renamePIDPID_sym_1 :
+  forall a b, renamePIDPID_sym a b a = b.
+Proof.
+  unfold renamePIDPID_sym. intros. by rewrite Nat.eqb_refl.
+Qed.
+
+Lemma well_formed_collapse :
+  forall l O n,
+    well_formed O n l ->
+    forall a, collapse_list l a.
+Proof.
+  induction l; intros; simpl.
+  trivial.
+  destruct a. inv H. eapply IHl in H3. split. 2: eassumption.
+  
+Qed.
+
+Lemma fresh_pid_list_is_not_in_step :
+  forall l O n n' a ι,
+  n -[ a | ι ]ₙ-> n' with O ->
+   well_formed O n l ->
+   collapse_list l a \/
+   (exists v1 v2 p', a = ASpawn p' v1 v2 /\ exists new, collapse_list ((p', new) :: l) a /\ well_formed O n ((p', new) :: l)).
+   (* p' ∈ (map snd l) /\ p' ∉ usedPIDsVal v1 ∪ usedPIDsVal v2) *)
+Proof.
+  induction l; intros; inv H0.
+  * left. constructor.
+  * eapply fresh_pid_is_not_in_step in H as P; eauto.
+    destruct P.
+    - destruct n' as [eth' Π']. eapply IHl with (a := renamePIDAct from to a0) in H3.
+      2: { apply renamePID_is_preserved_node_semantics; eauto.
+           by apply appearsEther_isUsedEther.
+         }
+      destruct H3.
+      + left. simpl. constructor. by simpl.
+        {
+          assumption.
+        }
+      + destruct_hyps. simpl in *.
+        destruct_hyps.
+        left. split. assumption.
+        destruct a0; inv H1.
+        simpl in *. admit.
+    - right. destruct_hyps. subst. do 3 eexists. split. reflexivity.
+      eexists. split.
+      + constructor.
+        ** simpl. admit. (* freshness *)
+        ** constructor; simpl.
+           -- rewrite renamePIDPID_1.
+              rewrite isNotUsed_renamePID_val. 2: set_solver.
+              rewrite isNotUsed_renamePID_val. 2: set_solver.
+              admit. (* freshness *)
+           -- repeat rewrite renamePIDPID_1.
+              repeat rewrite double_PIDrenaming_val.
+           
+      +
+Qed.
 
 
 Theorem rename_bisim :
+  forall O eth Π (l : list (PID * PID)),
+    ether_wf eth ->
+    (* Forall (fun p' => ¬ appearsEther p' eth) (map snd l) ->
+    (* p' ∉ dom Π -> *)
+    (* (p ∈ dom Π \/ (¬isUsedEther p eth /\ ¬isUsedPool p Π)) -> *)
+    (* (p ∈ dom Π \/ (¬isUsedEther p eth /\ ¬isUsedPool p Π)) -> *)
+    (* ~isUntaken p (eth, Π) -> *)
+    Forall (fun p' => ¬isUsedPool p' Π) (map snd l) ->
+    Forall (fun p => p ∉ O) (map fst l) ->
+    Forall (fun p => p ∉ O) (map snd l) -> *)
+    (* Forall (fun '(from, to) => ¬ appearsEther to eth /\ ¬isUsedPool to Π /\ to ∉ O /\ from ∉ O) l ->
+    NoDup (map snd l) -> *)
+    well_formed O (eth, Π) l ->
+    (eth, Π) ~ (renamePIDs renamePIDEther l eth, renamePIDs renamePIDPool l Π) observing O.
+Proof.
+  cofix IH.
+  intros. constructor; auto.
+  * apply renameList_preCompatible_sym. assumption.
+  * simpl. by apply ether_wf_renameList.
+  * intros. destruct A' as [eth' Π'].
+    (* eapply fresh_pid_list_is_not_in_step with (l := map snd l) in H1 as HD.
+    2: {
+      simpl. apply Forall_map. clear -H0.
+      eapply Forall_impl. eassumption. intros. destruct x; simpl in *.
+      set_solver.
+    }
+    destruct HD. *)
+    (* epose proof (List.Forall_Exists_dec (λ '(_, to), to ∉ usedPIDsAct a) _ l). *)
+    
+    Unshelve. 2: {
+      destruct x. simpl.
+      destruct (gset_elem_of_dec p0 (usedPIDsAct a)).
+      * right. set_solver.
+      * left. assumption.
+    }
+    destruct H2.
+    {
+      apply renamePIDlist_is_preserved_node_semantics with (l := l) in H1 as D.
+      3: clear IH; assumption.
+      2: {
+        (* clear IH; assumption. *) (* 
+        rewrite Forall_forall in f. rewrite Forall_forall in H3.
+        apply Forall_forall. intros. destruct x.
+        apply H0 in H4 as P1. destruct_hyps.
+        assert (p0 ∈ map snd l) by set_solver.
+        apply H3 in H9. split_and!; try assumption.
+        by apply appearsEther_isUsedEther.
+      } *)
+      }
+      do 2 eexists. split.
+      eapply n_trans. exact D. apply n_refl.
+      apply IH; clear IH.
+      * eapply n_trans in H1. 2:apply n_refl.
+        by apply ether_wf_preserved in H1.
+      * by eapply well_formed_preserved. (* 
+      * rewrite Forall_forall in H0. rewrite Forall_forall in H3.
+        apply Forall_forall. intros. destruct x.
+        apply H0 in H4 as P1. destruct_hyps.
+        assert (p0 ∈ map snd l) by set_solver.
+        apply H3 in H9. split_and!; try assumption.
+        eapply appearsEther_step in H2. exact H2. all: try assumption.
+        eapply not_isUsedPool_step in H2. exact H2. all: assumption.
+      * assumption. *)
+    }
+    { (* renaming is needed here *)
+      (* destruct H3 as [v1 [v2 [taken ?]]]. destruct_hyps.
+      subst. *)
+      rewrite Exists_exists in e. destruct e. destruct_hyps. destruct x.
+      assert (exists new, (* new ∉ map snd l /\
+                          new ∉ O /\
+                          ¬appearsEther new eth /\
+                          ¬isUsedPool new Π /\
+                          new ≠ taken /\
+                          new ∉ usedPIDsVal v1 ∪ usedPIDsVal v2 *)
+                          well_formed O (eth, Π) ((p0, new)::l)). {
+        clear IH. eexists. constructor; auto; admit.
+      }
+      destruct H4 as [new ?].
+      (* assert (Forall (fun p => p ∉ usedPIDsVal v1 ∪ usedPIDsVal v2) (map snd l)) as HP. {
+        (* the PIDs are not used in the spawn values which we use to rename with. *)
+        clear -H0 H2.
+        rewrite Forall_forall in H0. apply Forall_forall. intros.
+        rewrite elem_of_map_iff in H. destruct_hyps. destruct x0. simpl in *.
+        apply H0 in H1. subst. destruct_hyps.
+        apply fresh_pid_is_not_in_step with (p' := x) in H2; auto.
+        destruct H2. set_solver.
+        destruct_hyps. by inv H2.
+      } *)
+      apply renamePIDlist_is_preserved_node_semantics with (l := (p0, new) :: l) in H1 as D.
+      3: {
+        clear IH. assumption.
+      }
+      2: {
+      2: {
+        clear IH.
+        rewrite Forall_forall in H0.
+        apply Forall_forall. intros. destruct x.
+        apply elem_of_cons in H11 as [|].
+        * simpl. inv H11. split_and!; try assumption.
+          set_solver.
+          by apply appearsEther_isUsedEther.
+        * apply H0 in H11 as P1. destruct_hyps.
+          assert (p0 ∈ map snd l) by set_solver.
+          split_and!; try assumption.
+          - simpl. intros.
+            assert (p0 = taken \/ p0 ∈ usedPIDsVal v1 ∪ usedPIDsVal v2) as X by set_solver.
+            destruct X.
+            + subst. exists new. split_and!; auto.
+              apply elem_of_cons; by left. set_solver.
+            + exfalso. rewrite Forall_forall in HP. apply HP in H16. congruence.
+          - by apply appearsEther_isUsedEther.
+      }
+      replace (renamePIDs renamePIDEther l eth) with
+         (renamePIDs renamePIDEther ((taken, new)::l) eth). 2: {
+         simpl. rewrite does_not_appear_renamePID_ether; auto.
+         rewrite Forall_forall in H0. clear-H0 H4.
+         rewrite elem_of_map_iff in H4; destruct_hyps. destruct x.
+         simpl in *. apply H0 in H1. subst. apply H1.
+      }
+      replace (renamePIDs renamePIDPool l Π) with
+         (renamePIDs renamePIDPool ((taken, new)::l) Π). 2: {
+         simpl. rewrite isNotUsed_renamePID_pool; auto.
+         rewrite Forall_forall in H0. clear-H0 H4.
+         rewrite elem_of_map_iff in H4; destruct_hyps. destruct x.
+         simpl in *. apply H0 in H1. subst. apply H1.
+      }
+      do 2 eexists. split. eapply n_trans. exact D. apply n_refl.
+(*       replace (renamePIDs renamePIDEther ((taken, new) :: l) eth') with
+        (renamePIDs renamePIDEther ((taken, new) :: map (prod_map id (renamePIDPID_sym taken new) ) l) eth').
+            replace (renamePIDs renamePIDPool ((taken, new) :: l) Π') with
+        (renamePIDs renamePIDPool ((taken, new) :: map (prod_map id (renamePIDPID_sym taken new) ) l) Π'). *)
+      apply IH; clear IH.
+      * eapply n_trans in H2. 2:apply n_refl.
+        by apply ether_wf_preserved in H2.
+      * clear D.
+        rewrite Forall_forall in H0.
+        apply Forall_forall. intros. destruct x.
+        apply elem_of_cons in H11 as [|].
+        - simpl. inv H11. split_and!; try assumption.
+          eapply appearsEther_step in H2. exact H2. all: simpl.
+          set_solver.
+          assumption.
+          eapply not_isUsedPool_step in H2. eassumption. assumption.
+          simpl. set_solver.
+          rewrite elem_of_map_iff in H4. destruct_hyps. destruct x; subst.
+          simpl in *. apply H0 in H11. apply H11.
+        - apply elem_of_map_iff in H11. destruct_hyps. destruct x. inv H11.
+          apply H0 in H12 as D. destruct_hyps.
+          split_and!.
+          + destruct (decide (n = taken)).
+            ** subst. unfold renamePIDPID_sym. rewrite Nat.eqb_refl.
+               eapply appearsEther_step in H2. exact H2. set_solver. assumption.
+            ** assert (n ≠ new). {
+                 intro. subst. apply H3. apply elem_of_map_iff.
+                 eexists. split. 2: exact H12. reflexivity.
+               }
+               unfold renamePIDPID_sym. repeat case_match; eqb_to_eq; try congruence.
+               eapply appearsEther_step in H2. exact H2.
+               simpl. rewrite Forall_forall in HP.
+               assert (n ∈ map snd l). {
+                 apply elem_of_map_iff. eexists. split. 2: exact H12. reflexivity.
+               }
+               apply HP in H19. set_solver.
+               assumption.
+          + destruct (decide (n = taken)).
+            ** subst. unfold renamePIDPID_sym. rewrite Nat.eqb_refl.
+               eapply not_isUsedPool_step in H2. exact H2. assumption. set_solver.
+            ** assert (n ≠ new). {
+                 intro. subst. apply H3. apply elem_of_map_iff.
+                 eexists. split. 2: exact H12. reflexivity.
+               }
+               unfold renamePIDPID_sym. repeat case_match; eqb_to_eq; try congruence.
+               eapply not_isUsedPool_step in H2. exact H2. assumption.
+               simpl. rewrite Forall_forall in HP.
+               assert (n ∈ map snd l). {
+                 apply elem_of_map_iff. eexists. split. 2: exact H12. reflexivity.
+               }
+               apply HP in H19. set_solver.
+          + destruct (decide (n = taken)).
+            ** subst. unfold renamePIDPID_sym. rewrite Nat.eqb_refl. assumption.
+            ** assert (n ≠ new). {
+                 intro. subst. apply H3. apply elem_of_map_iff.
+                 eexists. split. 2: exact H12. reflexivity.
+               }
+               unfold renamePIDPID_sym. repeat case_match; eqb_to_eq; try congruence.
+          + assumption.
+      * simpl. constructor.
+        - rewrite map_map. intro. apply elem_of_map_iff in H11. destruct_hyps.
+          destruct x. simpl in *. unfold renamePIDPID_sym in H11.
+          repeat case_match; eqb_to_eq; subst; try congruence.
+          
+        -
+    }
+  * simpl. intros.
+    exists (renamePIDs renamePIDPID_sym l source), []. eexists.
+    split.
+    {
+      apply n_refl.
+    }
+    {
+      simpl.
+      assert ((renamePIDs renamePIDPID_sym l source, dest) =
+           ((prod_map (renamePIDs renamePIDPID_sym l) (renamePIDs renamePIDPID_sym l)) (source, dest))). {
+        cbn. f_equal. clear -H0 H1 H2.
+        generalize dependent dest.
+        induction l. reflexivity.
+        inv H1. inv H0. destruct a. simpl.
+        intros. rewrite <- IHl; auto.
+        * unfold renamePIDPID_sym.
+          destruct_hyps. repeat case_match;eqb_to_eq; subst; try congruence.
+        * unfold renamePIDPID_sym.
+          destruct_hyps. repeat case_match;eqb_to_eq; subst; try congruence.
+      }
+      setoid_rewrite H3.
+      {
+        clear. revert eth source dest.
+        induction l; intros; simpl.
+        * apply option_biforall_refl. intros. apply Signal_eq_refl.
+        * destruct a. eapply option_biforall_trans. 3: apply IHl.
+          - apply Signal_eq_trans.
+          - unfold renamePIDEther. replace (if source =? _ then _ else _, _) with
+              (prod_map (renamePIDPID_sym p p0) (renamePIDPID_sym p p0) (source, dest)) by reflexivity.
+            setoid_rewrite lookup_kmap; auto.
+            setoid_rewrite lookup_fmap.
+            simpl. destruct (eth !! _) eqn:P.
+            {
+              setoid_rewrite P. simpl.
+              eapply forall_biforall with (d1 := SUnlink) (d2 := SUnlink).
+              1: by rewrite map_length.
+              intros. rewrite map_nth with (d:= SUnlink).
+              by apply Signal_eq_renamePID.
+            }
+            {
+              setoid_rewrite P. simpl. trivial.
+            }
+      }
+    }
+  * admit.
+  * admit.
+Qed.
+
+
+
+
+
+
+
+
+
+
+
+
+
+
+
+
+
+
+
+Theorem rename_bisim_old :
   forall O eth Π (l : list (PID * PID)),
     ether_wf eth ->
     (* Forall (fun p' => ¬ appearsEther p' eth) (map snd l) ->
@@ -982,8 +1608,9 @@ Proof.
     destruct HD.
     {
       apply renamePIDlist_is_preserved_node_semantics with (l := l) in H2 as D.
-      3: assumption.
+      3: clear IH; assumption.
       2: {
+        clear IH.
         rewrite Forall_forall in H0. rewrite Forall_forall in H3.
         apply Forall_forall. intros. destruct x.
         apply H0 in H4 as P1. destruct_hyps.
@@ -993,7 +1620,7 @@ Proof.
       }
       do 2 eexists. split.
       eapply n_trans. exact D. apply n_refl.
-      apply IH.
+      apply IH; clear IH.
       * eapply n_trans in H2. 2:apply n_refl.
         by apply ether_wf_preserved in H2.
       * rewrite Forall_forall in H0. rewrite Forall_forall in H3.
@@ -1006,7 +1633,130 @@ Proof.
       * assumption.
     }
     { (* renaming is needed here *)
-      admit.
+      destruct H3 as [v1 [v2 [taken ?]]]. destruct_hyps.
+      subst.
+      assert (exists new, new ∉ map snd l /\
+                          new ∉ O /\
+                          ¬appearsEther new eth /\
+                          ¬isUsedPool new Π /\
+                          new ≠ taken /\
+                          new ∉ usedPIDsVal v1 ∪ usedPIDsVal v2). {
+        clear IH. admit.
+      }
+      destruct H3 as [new ?]. destruct_hyps.
+      assert (Forall (fun p => p ∉ usedPIDsVal v1 ∪ usedPIDsVal v2) (map snd l)) as HP. {
+        (* the PIDs are not used in the spawn values which we use to rename with. *)
+        clear -H0 H2.
+        rewrite Forall_forall in H0. apply Forall_forall. intros.
+        rewrite elem_of_map_iff in H. destruct_hyps. destruct x0. simpl in *.
+        apply H0 in H1. subst. destruct_hyps.
+        apply fresh_pid_is_not_in_step with (p' := x) in H2; auto.
+        destruct H2. set_solver.
+        destruct_hyps. by inv H2.
+      }
+      apply renamePIDlist_is_preserved_node_semantics_weakened with (l := (taken, new) :: l) in H2 as D.
+      3: {
+        clear IH. constructor; assumption.
+      }
+      2: {
+        clear IH.
+        rewrite Forall_forall in H0.
+        apply Forall_forall. intros. destruct x.
+        apply elem_of_cons in H11 as [|].
+        * simpl. inv H11. split_and!; try assumption.
+          set_solver.
+          by apply appearsEther_isUsedEther.
+        * apply H0 in H11 as P1. destruct_hyps.
+          assert (p0 ∈ map snd l) by set_solver.
+          split_and!; try assumption.
+          - simpl. intros.
+            assert (p0 = taken \/ p0 ∈ usedPIDsVal v1 ∪ usedPIDsVal v2) as X by set_solver.
+            destruct X.
+            + subst. exists new. split_and!; auto.
+              apply elem_of_cons; by left. set_solver.
+            + exfalso. rewrite Forall_forall in HP. apply HP in H16. congruence.
+          - by apply appearsEther_isUsedEther.
+      }
+      replace (renamePIDs renamePIDEther l eth) with
+         (renamePIDs renamePIDEther ((taken, new)::l) eth). 2: {
+         simpl. rewrite does_not_appear_renamePID_ether; auto.
+         rewrite Forall_forall in H0. clear-H0 H4.
+         rewrite elem_of_map_iff in H4; destruct_hyps. destruct x.
+         simpl in *. apply H0 in H1. subst. apply H1.
+      }
+      replace (renamePIDs renamePIDPool l Π) with
+         (renamePIDs renamePIDPool ((taken, new)::l) Π). 2: {
+         simpl. rewrite isNotUsed_renamePID_pool; auto.
+         rewrite Forall_forall in H0. clear-H0 H4.
+         rewrite elem_of_map_iff in H4; destruct_hyps. destruct x.
+         simpl in *. apply H0 in H1. subst. apply H1.
+      }
+      do 2 eexists. split. eapply n_trans. exact D. apply n_refl.
+      replace (renamePIDs renamePIDEther ((taken, new) :: l) eth') with
+        (renamePIDs renamePIDEther ((taken, new) :: map (prod_map id (renamePIDPID_sym taken new) ) l) eth').
+            replace (renamePIDs renamePIDPool ((taken, new) :: l) Π') with
+        (renamePIDs renamePIDPool ((taken, new) :: map (prod_map id (renamePIDPID_sym taken new) ) l) Π').
+      apply IH; clear IH.
+      * eapply n_trans in H2. 2:apply n_refl.
+        by apply ether_wf_preserved in H2.
+      * clear D.
+        rewrite Forall_forall in H0.
+        apply Forall_forall. intros. destruct x.
+        apply elem_of_cons in H11 as [|].
+        - simpl. inv H11. split_and!; try assumption.
+          eapply appearsEther_step in H2. exact H2. all: simpl.
+          set_solver.
+          assumption.
+          eapply not_isUsedPool_step in H2. eassumption. assumption.
+          simpl. set_solver.
+          rewrite elem_of_map_iff in H4. destruct_hyps. destruct x; subst.
+          simpl in *. apply H0 in H11. apply H11.
+        - apply elem_of_map_iff in H11. destruct_hyps. destruct x. inv H11.
+          apply H0 in H12 as D. destruct_hyps.
+          split_and!.
+          + destruct (decide (n = taken)).
+            ** subst. unfold renamePIDPID_sym. rewrite Nat.eqb_refl.
+               eapply appearsEther_step in H2. exact H2. set_solver. assumption.
+            ** assert (n ≠ new). {
+                 intro. subst. apply H3. apply elem_of_map_iff.
+                 eexists. split. 2: exact H12. reflexivity.
+               }
+               unfold renamePIDPID_sym. repeat case_match; eqb_to_eq; try congruence.
+               eapply appearsEther_step in H2. exact H2.
+               simpl. rewrite Forall_forall in HP.
+               assert (n ∈ map snd l). {
+                 apply elem_of_map_iff. eexists. split. 2: exact H12. reflexivity.
+               }
+               apply HP in H19. set_solver.
+               assumption.
+          + destruct (decide (n = taken)).
+            ** subst. unfold renamePIDPID_sym. rewrite Nat.eqb_refl.
+               eapply not_isUsedPool_step in H2. exact H2. assumption. set_solver.
+            ** assert (n ≠ new). {
+                 intro. subst. apply H3. apply elem_of_map_iff.
+                 eexists. split. 2: exact H12. reflexivity.
+               }
+               unfold renamePIDPID_sym. repeat case_match; eqb_to_eq; try congruence.
+               eapply not_isUsedPool_step in H2. exact H2. assumption.
+               simpl. rewrite Forall_forall in HP.
+               assert (n ∈ map snd l). {
+                 apply elem_of_map_iff. eexists. split. 2: exact H12. reflexivity.
+               }
+               apply HP in H19. set_solver.
+          + destruct (decide (n = taken)).
+            ** subst. unfold renamePIDPID_sym. rewrite Nat.eqb_refl. assumption.
+            ** assert (n ≠ new). {
+                 intro. subst. apply H3. apply elem_of_map_iff.
+                 eexists. split. 2: exact H12. reflexivity.
+               }
+               unfold renamePIDPID_sym. repeat case_match; eqb_to_eq; try congruence.
+          + assumption.
+      * simpl. constructor.
+        - rewrite map_map. intro. apply elem_of_map_iff in H11. destruct_hyps.
+          destruct x. simpl in *. unfold renamePIDPID_sym in H11.
+          repeat case_match; eqb_to_eq; subst; try congruence.
+          
+        -
     }
   * simpl. intros.
     exists (renamePIDs renamePIDPID_sym l source), []. eexists.
@@ -1029,24 +1779,29 @@ Proof.
           destruct_hyps. repeat case_match;eqb_to_eq; subst; try congruence.
       }
       setoid_rewrite H3.
-      
-      -------------------------------------------------------- PROGRESS HERE
-      
-      
-      setoid_rewrite lookup_kmap; auto.
-      setoid_rewrite lookup_fmap.
-      simpl. destruct (eth !! _) eqn:P.
       {
-        setoid_rewrite P. simpl.
-        eapply forall_biforall with (d1 := SUnlink) (d2 := SUnlink).
-        1: by rewrite map_length.
-        intros. rewrite map_nth with (d:= SUnlink).
-        by apply Signal_eq_renamePID.
+        clear. revert eth source dest.
+        induction l; intros; simpl.
+        * apply option_biforall_refl. intros. apply Signal_eq_refl.
+        * destruct a. eapply option_biforall_trans. 3: apply IHl.
+          - apply Signal_eq_trans.
+          - unfold renamePIDEther. replace (if source =? _ then _ else _, _) with
+              (prod_map (renamePIDPID_sym p p0) (renamePIDPID_sym p p0) (source, dest)) by reflexivity.
+            setoid_rewrite lookup_kmap; auto.
+            setoid_rewrite lookup_fmap.
+            simpl. destruct (eth !! _) eqn:P.
+            {
+              setoid_rewrite P. simpl.
+              eapply forall_biforall with (d1 := SUnlink) (d2 := SUnlink).
+              1: by rewrite map_length.
+              intros. rewrite map_nth with (d:= SUnlink).
+              by apply Signal_eq_renamePID.
+            }
+            {
+              setoid_rewrite P. simpl. trivial.
+            }
       }
-      {
-        setoid_rewrite P. simpl. trivial.
-      }
-    } *)
+    }
   * admit.
   * admit.
 Qed.
