src/Concurrent/InductiveNodeSemantics.v
@@ -3301,3 +3301,4 @@ Corollary renamePID_id_pool :
 Proof.
 
 Admitted.
+
